theories/Sim.v
@@ -1,0 +1,135 @@
+From Stdlib Require Import Utf8.
+
+From Stdlib Require Import Lists.List.
+From Stdlib Require Import Strings.String.
+From Stdlib Require Import ZArith.ZArith.
+From Stdlib Require Import Lia.
+
+From stdpp Require Import relations.
+From stdpp Require Import tactics.
+
+From RSL Require Import RTL.
+From RSL Require Import Notations.
+From RSL Require Import Semantics.
+From RSL Require Import Logic.
+From RSL Require Import WP.
+
+Import RTLNotations.
+Import ListNotations.
+
+Section Sim.
+  Variable P: program.
+
+  Definition exec : Type := nat → state.
+
+  (** Asserts that f is a diverging execution from s. *)
+  Definition diverging_execution (f: exec) (s: state) :=
+    f 0 = s ∧ ∀ n, P ⊨ f n ->> f (S n).
+
+  (** s is a diverging state if s is the begining of some diverging execution *)
+  Definition diverges (s: state) := ∃ f, diverging_execution f s.
+
+  Variant behavior :=
+  | Terminating (v: val) (m: memory)
+  | Diverging
+  | Unknown.
+
+  Inductive behavior_order : behavior -> behavior -> Prop :=
+  | TerminatingOrder : ∀ v m, behavior_order (Terminating v m) (Terminating v m)
+  | DivergingOrder : behavior_order Diverging Diverging
+  | UnkownOrder : ∀ s, behavior_order s Unknown.
+
+  Instance behavior_order_inst : PartialOrder behavior_order.
+  Proof.
+    split. 1: split.
+    - intros []; constructor.
+    - intros x y z Hxy Hyz. inv Hxy.
+      + assumption.
+      + assumption.
+      + inv Hyz. constructor.
+    - intros x y Hxy Hyx. inv Hxy; try reflexivity.
+      now inv Hyx.
+  Qed.
+  Instance behavior_order_notation : SqSubsetEq behavior := behavior_order.
+
+  (* [beh s] is the set of all the behaviors of [s] *)
+  Inductive beh : state -> behavior -> Prop :=
+  | IsTerminating : ∀ v m,
+      beh ([], ReturnState v, m) (Terminating v m)
+  | IsDiverging : ∀ s,
+      diverges s ->
+      beh s Diverging
+  | IsStuck : ∀ s,
+      stuck P s ->
+      beh s Unknown
+  | IsSteping : ∀ s t b,
+      beh t b ->
+      P ⊨ s ->> t ->
+      beh s b.
+
+  Instance beh_elem_state : ElemOf behavior (behavior -> Prop) := fun b P => P b.
+
+  (* [s] is terminating iff there is a execution from [s] to a final state. *)
+  Lemma has_terminating_behavior : ∀ s v m,
+    Terminating v m ∈ beh s <-> P ⊨ s ->>* ([], ReturnState v, m).
+  Proof.
+    intros s v m. split; intros H.
+    - remember (Terminating v m) as b eqn:Hb.
+      induction H as [ | | | s t b ? IH Hstep ] in s, H, v, m, b, Hb |- *; inv Hb.
+      + constructor.
+      + apply rtc_l with t; now auto.
+    - remember ([], ReturnState v, m) as t eqn:Ht.
+      induction H as [ | s t u Hstep Hrtc IH ]
+        in t, Ht, v, m, H |- *; subst.
+      + constructor.
+      + econstructor. 2: eassumption. firstorder.
+  Qed.
+
+  (* [s] is diverging iff [s] has a diverging execution *)
+  Lemma has_diverging_behavior : ∀ s,
+    Diverging ∈ beh s <-> diverges s.
+  Proof.
+    intros s. split; intros H.
+    - remember Diverging as b eqn:Hb.
+      induction H as [ | | | s t b ? IH Hstep ]
+        in s, b, Hb, H |- *; try discriminate Hb; eauto.
+      destruct (IH Hb) as (f & Hinit & Hsucc).
+      exists (fun n => match n with O => s | S n => f n end). split.
+      + reflexivity.
+      + intros []; now subst.
+    - now constructor.
+  Qed.
+
+  (* [s] has a unknown behavior if [s] reduces to a stuck state. *)
+  Lemma has_stuck_behavior : ∀ s,
+    Unknown ∈ beh s <-> ∃ t, P ⊨ s ->>* t ∧ stuck P t.
+  Proof.
+    intros s. split; intros H.
+    - remember Unknown as b eqn:Hb.
+      induction H as [ s | | | s t b ? IH Hstep ]
+        in s, b, Hb, H |- *; try discriminate Hb; eauto.
+      + exists s. now split.
+      + destruct (IH Hb) as (u & Hrtc & Hstuck).
+        exists u. split.
+        * now apply rtc_l with t.
+        * assumption.
+    - destruct H as (u & Hrtc & Hstuck).
+      induction Hrtc  as [ | s t u Hstep Hrtc IH] in s, u, Hrtc, Hstuck |- *.
+      + now constructor.
+      + eapply IsSteping.
+        * now apply IH.
+        * easy.
+  Qed.
+
+  (* A definition of state refinement:
+     - if the target terminates on (v, m),
+       the source must either terminate on (v, m) or be stuck.
+     - if the target diverges,
+       the source must either diverges or be stuck.
+     - if the target is stuck, the source should also be stuck.
+   *)
+  Definition refines (t: state) (s: state) :=
+    ∀ b, b ∈ beh t -> ∃ b', b' ∈ beh s ∧ b ⊑ b'.
+
+
+End Sim.
